Generalize declaration of top-level regions

src/tls/Mem.fst
@@ -126,30 +126,89 @@ let tls_region: tls_rgn = new_colored_region HS.root tls_color
 
 type subtls = r: subrgn tls_region {is_tls_rgn r} 
 
-noextract
-private let p :
-  r0:subtls &
-  r1:subtls &
-  r2:subtls
-  {r1 `disjoint` r0 /\ r2 `disjoint` r0 /\ r2 `disjoint` r1} =
-  let r0 = new_colored_region tls_region tls_color in
-  let r1 = new_colored_region tls_region tls_color in
-  let r2 = new_colored_region tls_region tls_color in
-  (| r0, r1, r2 |)
+val rlist_disjoint0: subtls -> l:list subtls -> Tot Type0 (decreases %[l;0])
+val r_pairwise_disjoint0: l:list subtls -> Tot Type0 (decreases %[l;1])
+val r_fresh0: l:list subtls -> h0:mem -> h1:mem -> Tot Type0 (decreases %[l])
 
-// consider dropping the tls_ prefix
-noextract
-let tls_tables_region: r:tls_rgn =
-  match p with | (| r, _, _ |) -> r
+let rec rlist_disjoint0 r = function
+  | [] -> True
+  | h::t -> h `disjoint` r /\ (rlist_disjoint0 r t)
 
-noextract
-let tls_define_region: r:tls_rgn{r `disjoint` tls_tables_region} =
-  match p with | (| _, r, _ |) -> r
+let rec r_pairwise_disjoint0 = function
+  | [] -> True
+  | h::t -> rlist_disjoint0 h t /\ r_pairwise_disjoint0 t
 
-noextract
-let tls_honest_region: r:tls_rgn{r `disjoint` tls_tables_region /\ r `disjoint` tls_define_region} =
-  match p with | (| _, _, r |) -> r
+let rec r_fresh0 l h0 h1 =
+  match l with
+  | [] -> True
+  | r :: t -> fresh_region r h0 h1 /\ r_fresh0 t h0 h1
 
+unfold let rlist_disjoint r l = normalize_term (rlist_disjoint0 r l)
+unfold let r_pairwise_disjoint l = normalize_term (r_pairwise_disjoint0 l)
+unfold let r_fresh l = normalize_term (r_fresh0 l)
+
+let lemma_fresh_back (r:rgn) (h0 h1 h2:mem)
+  : Lemma (requires fresh_region r h1 h2 /\ modifies_none h0 h1)
+  (ensures fresh_region r h0 h2)
+  = ()
+
+let rec lemma_r_fresh_disjoint (r:subtls) (l:list subtls) (h0 h1 h2:mem)
+  : Lemma
+    (requires r_fresh0 l h0 h1 /\ fresh_region r h1 h2 /\ modifies_none h0 h1)
+    (ensures rlist_disjoint0 r l)
+  =
+  match l with
+  | [] -> ()
+  | x::t -> lemma_extends_disjoint tls_region r x;
+    lemma_r_fresh_disjoint r t h0 h1 h2
+
+let rec rdisjoint_alloc (n:nat) :
+  ST (l:list subtls)
+  (requires fun h0 -> True)
+  (ensures fun h0 l h1 ->
+    modifies_none h0 h1 /\
+    r_fresh0 l h0 h1 /\
+    List.Tot.length l == n /\
+    r_pairwise_disjoint0 l)
+  =
+  if n = 0 then []
+  else
+   begin
+    let h0 = get () in
+    let t = rdisjoint_alloc (n-1) in
+    let h1 = get () in
+    let h = new_colored_region tls_region tls_color in
+    let h2 = get () in
+    assume(r_fresh0 t h0 h2);
+    lemma_r_fresh_disjoint h t h0 h1 h2;
+    h :: t
+   end
+
+// We use region disjintness as a coarse grained way
+// of framing invariants.
+let top_regions: (l:list subtls{List.Tot.length l == 5 /\ r_pairwise_disjoint0 l})
+  = rdisjoint_alloc 5
+let _ = assert(List.Tot.length top_regions == 5)
+
+let tls_tables_region = List.Tot.index top_regions 0
+let tls_define_region = List.Tot.index top_regions 1
+let tls_honest_region = List.Tot.index top_regions 2
+let tls_psk_region = List.Tot.index top_regions 3
+let tls_crf_region = List.Tot.index top_regions 4
+
+// OK but requires ifuel to unfold rdisjoint
+let _ = assert(tls_define_region `disjoint` tls_psk_region)
+
+// FIXME(adl) annoying, but easy
+let lemma_top_regions_disjoint (i j:nat)
+  : Lemma (requires i < 5 /\ j < 5 /\ i <> j)
+  (ensures (List.Tot.index top_regions i) `disjoint` (List.Tot.index top_regions j))
+  [SMTPat (List.Tot.index top_regions i); SMTPat (List.Tot.index top_regions j)]
+  = admit()
+
+// Sanity check. The lemma should give disjointness even without fuel
+#set-options "--max_fuel 0 --max_ifuel 0"
+let _ = assert(tls_crf_region `disjoint` tls_tables_region)
 
 // used for defining 1-shot PRFs and authenticators
 //18-01-04 could be promoted to Preorder 
@@ -179,3 +238,29 @@ let fresh_is_disjoint (old_loc:M.loc) (new_loc:M.loc)
 
 type sub_loc (parent:M.loc) =
   l:M.loc{if model then M.loc_includes parent l else l == M.loc_none}
+
+// Loc versions of above regions.
+let loc_tables_region = M.loc_region_only true tls_tables_region
+let loc_define_region = M.loc_region_only true tls_define_region
+let loc_honest_region = M.loc_region_only true tls_honest_region
+let loc_psk_region = M.loc_region_only true tls_psk_region
+let loc_crf_region = M.loc_region_only true tls_crf_region
+
+let lemma_disjoint_regions (r1 r2:subtls)
+  : Lemma (requires r1 `disjoint` r2)
+  (ensures (M.loc_region_only true r1) `M.loc_disjoint` (M.loc_region_only true r2))
+  = ()
+
+let lemma_top_loc_disjoint (i j:nat)
+  : Lemma (requires i < 5 /\ j < 5 /\ i <> j)
+  (ensures (M.loc_region_only true (List.Tot.index top_regions i)) `M.loc_disjoint` (M.loc_region_only true (List.Tot.index top_regions j)))
+  [SMTPat (M.loc_region_only true (List.Tot.index top_regions i)); SMTPat (M.loc_region_only true (List.Tot.index top_regions j))]
+  = ()
+
+(*
+FIXME(adl)
+#set-options "--max_fuel 2 --max_ifuel 2"
+let _ =
+  lemma_disjoint_regions tls_tables_region tls_define_region;
+  assert(loc_tables_region `M.loc_disjoint` loc_define_region)
+*)
